Fairness/All.v
@@ -3,4 +3,4 @@
 	Convenience re-export of the fairness formulas and mechanically-checked
 	theorems.
 *)
-From Fairness Require Export Interpretation PriorityFairness QuantityFairness PriceFairness MatchFinality Maximality JustifiedRejection.
+From Fairness Require Export Interpretation PriorityFairness QuantityFairness PriceFairness.
