LTL/LTL.v
@@ -1,3 +1,3 @@
 (* LTL/LTL.v *)
-From LTL Require Export Syntax Semantics Axioms Soundness Completeness.
+From LTL Require Export Syntax Semantics.
 Local Open Scope LTL_scope.
